theories/FreeVariables.v
@@ -1,0 +1,292 @@
+From Coq Require Export
+  Lists.List.
+Export ListNotations.
+From Lang Require Import
+  Invert
+  Mint
+  OptionBind
+  Snoc
+  Terms.
+
+Fixpoint remove_all x li :=
+  match li with
+  | [] => []
+  | hd :: tl =>
+      let recursed := remove_all x tl in
+      if eqb x hd then recursed else hd :: recursed
+  end.
+(* tail-recursive version flips the order *)
+
+Definition remove_if_head x li :=
+  match li with
+  | [] => []
+  | hd :: tl => if eqb x hd then tl else li
+  end.
+Arguments remove_if_head/ x li.
+
+Fixpoint fv_slow t :=
+  match t with
+  | TmVoid
+  | TmStar _
+  | TmAtom _ =>
+      []
+  | TmVarS s =>
+      [s]
+  | TmAppl f x =>
+      fv_slow f ++ fv_slow x
+  | TmPack _ arg ty curry
+  | TmForA arg ty curry =>
+      fv_slow ty ++ (
+        let recursed := fv_slow curry in
+        match arg with
+        | None => recursed
+        | Some a => (if mint ty then remove_all else remove_if_head) a recursed
+        end)
+  end.
+
+(* Crucial distinction from an easier-to-implement algorithm! *)
+Example fv_slow_permits_shadowing : forall x,
+  (* Equivalent to `\x. \x. x x`, where the `x`s are distinct and pushed/popped in order. *)
+  fv_slow (TmForA (Some x) TmVoid (TmForA (Some x) TmVoid (TmAppl (TmVarS x) (TmVarS x)))) = [].
+Proof. intros. simpl. repeat rewrite eqb_refl. reflexivity. Qed.
+
+(* Crucial distinction from an easier-to-implement algorithm! *)
+Example fv_slow_permits_interrupted_shadowing : forall x y, y <> x ->
+  (* Equivalent to `\x. \y. \x. x x`, where the `x`s are distinct and pushed/popped in order. *)
+  fv_slow (TmForA (Some x) TmVoid (TmForA (Some y) TmVoid (TmForA (Some x) TmVoid (TmAppl (TmVarS x) (TmVarS x))))) = [].
+Proof. intros. apply eqb_neq in H. simpl. rewrite eqb_refl. reflexivity. Qed.
+
+Example fv_slow_respects_scope : forall x,
+  (* Equivalent to `(\x:0. 0) x`, in which the outer `x` is still free *)
+  fv_slow (TmAppl (TmForA (Some x) TmVoid TmVoid) (TmVarS x)) = [x].
+Proof. intros. simpl. reflexivity. Qed.
+
+Fixpoint fv_fast acc t :=
+  match t with
+  | TmVoid
+  | TmStar _
+  | TmAtom _ =>
+      acc
+  | TmVarS s =>
+      s :: acc
+  | TmPack _ None a b
+  | TmForA None a b
+  | TmAppl a b =>
+      fv_fast (fv_fast acc b) a
+  | TmPack _ (Some arg) ty curry
+  | TmForA (Some arg) ty curry =>
+      fv_fast (remove_if_head arg (fv_fast acc curry)) ty
+  end.
+
+(* Crucial distinction from an easier-to-implement algorithm! *)
+Example fv_fast_permits_shadowing : forall x,
+  (* Equivalent to `\x. \x. x x`, where the `x`s are distinct and pushed/popped in order. *)
+  fv_fast [] (TmForA (Some x) TmVoid (TmForA (Some x) TmVoid (TmAppl (TmVarS x) (TmVarS x)))) = [].
+Proof. intros. simpl. repeat rewrite eqb_refl. reflexivity. Qed.
+
+(* Crucial distinction from an easier-to-implement algorithm! *)
+Example fv_fast_permits_interrupted_shadowing : forall x y, y <> x ->
+  (* Equivalent to `\x. \y. \x. x x`, where the `x`s are distinct and pushed/popped in order. *)
+  fv_fast [] (TmForA (Some x) TmVoid (TmForA (Some y) TmVoid (TmForA (Some x) TmVoid (TmAppl (TmVarS x) (TmVarS x))))) = [].
+Proof. intros. apply eqb_neq in H. simpl. rewrite eqb_refl. rewrite H. rewrite eqb_refl. reflexivity. Qed.
+
+Example fv_fast_respects_scope : forall x,
+  (* Equivalent to `(\x:0. 0) x`, in which the outer `x` is still free *)
+  fv_fast [] (TmAppl (TmForA (Some x) TmVoid TmVoid) (TmVarS x)) = [x].
+Proof. intros. simpl. Abort.
+
+(*
+Theorem fv_fast_slow_eq : forall t,
+  fv_slow t = rev (snd (fv_fast [] [] t)).
+Proof.
+  intros t. induction t; intros; simpl in *; try reflexivity.
+  - destruct arg.
+    + destruct (fv_slow t2).
+      * rewrite app_nil_r. rewrite IHt1. destruct (fv_fast [] [] t1).
+Qed.
+
+Definition fv := fv_fast [].
+*)
+
+Definition fv := fv_slow.
+Arguments fv/ t.
+
+(* Crucial distinction from an easier-to-implement algorithm! *)
+Example fv_permits_shadowing : forall x,
+  (* Equivalent to `\x. \x. x x`, where the `x`s are distinct and pushed/popped in order. *)
+  fv (TmForA (Some x) TmVoid (TmForA (Some x) TmVoid (TmAppl (TmVarS x) (TmVarS x)))) = [].
+Proof. intros. simpl. repeat rewrite eqb_refl. reflexivity. Qed.
+
+(* Crucial distinction from an easier-to-implement algorithm! *)
+Example fv_permits_interrupted_shadowing : forall x y, y <> x ->
+  (* Equivalent to `\x. \y. \x. x x`, where the `x`s are distinct and pushed/popped in order. *)
+  fv (TmForA (Some x) TmVoid (TmForA (Some y) TmVoid (TmForA (Some x) TmVoid (TmAppl (TmVarS x) (TmVarS x))))) = [].
+Proof. intros. apply eqb_neq in H. simpl. rewrite eqb_refl. reflexivity. Qed.
+
+Example fv_respects_scope : forall x,
+  (* Equivalent to `(\x:0. 0) x`, in which the outer `x` is still free *)
+  fv (TmAppl (TmForA (Some x) TmVoid TmVoid) (TmVarS x)) = [x].
+Proof. intros. simpl. reflexivity. Qed.
+
+Inductive Wherever {T} (x : T) : list T -> list T -> Prop :=
+  | WhereverNil :
+      Wherever x [] []
+  | WhereverHere : forall a b,
+      Wherever x a b ->
+      Wherever x a (x :: b)
+  | WhereverSkip : forall hd tla tlb,
+      x <> hd ->
+      Wherever x tla tlb ->
+      Wherever x (hd :: tla) (hd :: tlb)
+  .
+
+Example wherever_12345 : Wherever 9 [1;2;3;4;5] [9;1;9;9;2;3;9;4;9;9;9;9;5;9].
+Proof. repeat constructor; intro C; discriminate C. Qed.
+
+Lemma wherever_refl : forall {T} (x : T) li,
+  (~In x li) ->
+  Wherever x li li.
+Proof.
+  induction li; constructor; apply Decidable.not_or in H as [H I]. { symmetry. assumption. } apply IHli. assumption.
+Qed.
+
+Lemma wherever_not_in_orig : forall {T} (x : T) li post,
+  Wherever x li post ->
+  ~In x li.
+Proof.
+  intros T x li post H C. generalize dependent C. generalize dependent post. generalize dependent x.
+  induction li; intros; destruct C; subst.
+  - remember (x :: li) as xli eqn:Ex. induction H; intros.
+    { discriminate. } { apply IHWherever. assumption. } invert Ex. apply H. reflexivity.
+  - remember (a :: li) as ali eqn:Ea. generalize dependent a. generalize dependent li. induction H; intros.
+    { discriminate. } { eapply IHWherever. { apply IHli. } { assumption. } apply Ea. }
+    invert Ea. eapply IHli. { apply H0. } assumption.
+Qed.
+
+Lemma wherever_remove_all : forall x li post,
+  Wherever x li post <-> remove_all x post = li.
+Proof.
+  split; intros.
+  - induction H.
+    + reflexivity.
+    + simpl. rewrite eqb_refl. assumption.
+    + simpl. apply eqb_neq in H. rewrite H. f_equal. assumption.
+  - generalize dependent x. generalize dependent li. induction post; intros.
+    + invert H. constructor.
+    + simpl in H. destruct (eqb x a) eqn:E.
+      * apply eqb_eq in E. subst. constructor. apply IHpost. reflexivity.
+      * apply eqb_neq in E. subst. constructor. { assumption. } apply IHpost. reflexivity.
+Qed.
+
+Inductive FreeIn : term -> list string -> Prop :=
+  | FreeVoid :
+      FreeIn TmVoid []
+  | FreeStar : forall univ,
+      FreeIn (TmStar univ) []
+  | FreeAtom : forall id,
+      FreeIn (TmAtom id) []
+  | FreeVarS : forall x,
+      FreeIn (TmVarS x) [x]
+  | FreePackNone : forall id ty curry va vb v,
+      FreeIn ty va ->
+      FreeIn curry vb ->
+      va ++ vb = v ->
+      FreeIn (TmPack id None ty curry) v
+  | FreeForANone : forall ty curry va vb v,
+      FreeIn ty va ->
+      FreeIn curry vb ->
+      va ++ vb = v ->
+      FreeIn (TmForA None ty curry) v
+  | FreeAppl : forall f x va vb v,
+      FreeIn f va ->
+      FreeIn x vb ->
+      va ++ vb = v ->
+      FreeIn (TmAppl f x) v
+  | FreePackMint : forall id arg ty curry va vb avb v,
+      Mint ty ->
+      FreeIn ty va ->
+      FreeIn curry avb ->
+      Wherever arg vb avb ->
+      va ++ vb = v ->
+      FreeIn (TmPack id (Some arg) ty curry) v
+  | FreeForAMint : forall arg ty curry va vb avb v,
+      Mint ty ->
+      FreeIn ty va ->
+      FreeIn curry avb ->
+      Wherever arg vb avb ->
+      va ++ vb = v ->
+      FreeIn (TmForA (Some arg) ty curry) v
+  | FreePackMatch : forall id arg ty curry va vb v,
+      ~Mint ty ->
+      FreeIn ty va ->
+      FreeIn curry (arg :: vb) ->
+      va ++ vb = v ->
+      FreeIn (TmPack id (Some arg) ty curry) v
+  | FreeForAMatch : forall arg ty curry va vb v,
+      ~Mint ty ->
+      FreeIn ty va ->
+      FreeIn curry (arg :: vb) ->
+      va ++ vb = v ->
+      FreeIn (TmForA (Some arg) ty curry) v
+  | FreePackDiff : forall id arg ty curry va vb v,
+      ~Mint ty ->
+      FreeIn ty va ->
+      FreeIn curry vb ->
+      va ++ vb = v ->
+      hd_error vb <> Some arg ->
+      FreeIn (TmPack id (Some arg) ty curry) v
+  | FreeForADiff : forall arg ty curry va vb v,
+      ~Mint ty ->
+      FreeIn ty va ->
+      FreeIn curry vb ->
+      va ++ vb = v ->
+      hd_error vb <> Some arg ->
+      FreeIn (TmForA (Some arg) ty curry) v
+  .
+(* TODO: consider making these `Mint`s their Boolean equivalents, since manually calling constructors is a pain in the ass *)
+
+Definition Closed := fun t => FreeIn t [].
+Arguments Closed t/.
+
+Lemma map_distr : forall {A B} (f : A -> B) hd tl, map f (hd ++ tl) = map f hd ++ map f tl.
+Proof.
+  intros. generalize dependent tl. generalize dependent B.
+  induction hd; intros; simpl in *; try rewrite IHhd; reflexivity.
+Qed.
+
+Theorem reflect_fv : forall t v,
+  FreeIn t v <-> fv t = v.
+Proof.
+  split; intros.
+  - induction H; intros; subst; simpl in *; f_equal.
+    + apply mint_true in H. rewrite H. apply wherever_remove_all. assumption.
+    + apply mint_true in H. rewrite H. apply wherever_remove_all. assumption.
+    + apply mint_false in H. rewrite H. rewrite IHFreeIn2. rewrite eqb_refl. reflexivity.
+    + apply mint_false in H. rewrite H. rewrite IHFreeIn2. rewrite eqb_refl. reflexivity.
+    + apply mint_false in H. rewrite H. destruct (fv_slow curry). { reflexivity. }
+      destruct (eqb arg s) eqn:E. { apply eqb_eq in E. subst. contradiction H3. reflexivity. } reflexivity.
+    + apply mint_false in H. rewrite H. destruct (fv_slow curry). { reflexivity. }
+      destruct (eqb arg s) eqn:E. { apply eqb_eq in E. subst. contradiction H3. reflexivity. } reflexivity.
+  - generalize dependent v. induction t; intros; subst; simpl in *; try solve [constructor].
+    + destruct arg.
+      * destruct (reflect_mint t1). {
+          eapply FreePackMint; [assumption | apply IHt1 | apply IHt2 | apply wherever_remove_all |]; try reflexivity. }
+        destruct (fv_slow t2). {
+          eapply FreePackDiff; [assumption | apply IHt1 | apply IHt2 | |]; try reflexivity. intro C. discriminate C. }
+        destruct (eqb s s0) eqn:E. {
+          apply eqb_eq in E. subst. eapply FreePackMatch; [assumption | apply IHt1 | apply IHt2 |]; reflexivity. }
+        eapply FreePackDiff; [assumption | apply IHt1 | apply IHt2 | |]; try reflexivity.
+        intro C. invert C. rewrite eqb_refl in E. discriminate E.
+      * econstructor; [apply IHt1 | apply IHt2 |]; reflexivity.
+    + destruct arg.
+      * destruct (reflect_mint t1). {
+          eapply FreeForAMint; [assumption | apply IHt1 | apply IHt2 | apply wherever_remove_all |]; try reflexivity. }
+        destruct (fv_slow t2). {
+          eapply FreeForADiff; [assumption | apply IHt1 | apply IHt2 | |]; try reflexivity. intro C. discriminate C. }
+        destruct (eqb s s0) eqn:E. {
+          apply eqb_eq in E. subst. eapply FreeForAMatch; [assumption | apply IHt1 | apply IHt2 |]; reflexivity. }
+        eapply FreeForADiff; [assumption | apply IHt1 | apply IHt2 | |]; try reflexivity.
+        intro C. invert C. rewrite eqb_refl in E. discriminate E.
+      * econstructor; [apply IHt1 | apply IHt2 |]; reflexivity.
+    + econstructor; [apply IHt1 | apply IHt2 |]; reflexivity.
+Qed.
